src/lib/inst/gemm/Kuiper.GEMM.BlockTiling2D.fsti
@@ -1,0 +1,13 @@
+module Kuiper.GEMM.BlockTiling2D
+
+#lang-pulse
+open Kuiper
+open Kuiper.Poly.GEMMCPU
+open Kuiper.Matrix.Reprs { row_major as RM, col_major as CM }
+
+(* NOTE: no dynamic tile version as that would imply the use of a
+   stack-allocated variable-length array, and NVCC complains
+   (karamel warns too). *)
+
+val matmul_f32_64x8x64_8x8_rrr : fixed_repr_matmul_cpu_ty f32 RM RM RM
+val matmul_f32_32x32x32_32x8_rrr : fixed_repr_matmul_cpu_ty f32 RM RM RM
